lemma lecture11: manual; progress; admit (*WIP*). And archived some notes

lecture-files-fixed/Lecture_11/Solution11.ec
@@ -4,28 +4,40 @@
 
 pragma Goals:printall.
 
-require import Int.
-require import Real.
-require import Bool.
-require import Option.
+require import AllCore.
 require import Distr.
-require import ISet.
 require import List.
 require ROM.
-
-pragma Goals:printall.
-
+require import FSet.
+require import SmtMap.
 
 type K.
 type M. (* messages *)
 type Mblock. (* PRF input *)
 type C. (* output of PRF and random function *)
 
-axiom Mblockfin: Finite.finite univ<:Mblock>.
-axiom Cfin: Finite.finite univ<:C>.
-axiom Kfin: Finite.finite univ<:K>.
+clone Distr.MFinite as KS with
+  type t <= K.
 
-op unif = FSet.Duni.duni (ISet.Finite.toFSet ISet.univ<:'a>).
+clone Distr.MFinite as MBS with
+  type t <= Mblock.
+
+clone Distr.MFinite as CTS with
+  type t <= C.
+
+clone Distr.MFinite as MBlockToC with
+type t <= Mblock -> C.
+
+(* 
+Here we are axiomatizing the finiteness of multiple things.
+First we axiomatize the finiteness of different data-types.
+Next, we are axiomatizing the finiteness of the functions that map Mblock -> C.
+This is still "cheating". If we didn't want to cheat, we would need to
+prove multiple things.
+We looked at how we could do this in Lecture 4, however we are trying to learn
+how to work with cryptographic protocols so we will proceed with the
+axiomatic approach.
+*)
 
 (* Definition of PRFs *)
 
@@ -37,7 +49,7 @@ module type PRFOracleT = {
 }.
 
 module type AdvPRF(O:PRFOracleT) = {
-  proc guess(q:int): bool  (* Adv gets max number of queries *)
+    proc guess(q:int): bool (* Adv gets max number of queries *)
 }.
 
 module PRFOracle:PRFOracleT = {
@@ -47,11 +59,11 @@ module PRFOracle:PRFOracleT = {
 
   proc queryPRF(m:Mblock) : C = {
       var r;
-      if (num_q >= max_q) {
-        r = witness;
+      if (max_q <= num_q) {
+        r <- witness;
       } else {
-        num_q = num_q + 1;
-        r = f m;
+        num_q <- num_q + 1;
+        r <- f m;
       }
       
       return r;
@@ -63,24 +75,23 @@ module PRF_Game1(A : AdvPRF) = {
 
   proc main(q0:int) : bool = {
     var k, b;
-    k = $ unif;
-    PRFOracle.f = prf k;
-    PRFOracle.max_q = q0;
-    PRFOracle.num_q = 0;
+    k <$ KS.dunifin;
+    PRFOracle.f <- prf k;
+    PRFOracle.max_q <- q0;
+    PRFOracle.num_q <- 0;
     
-    b = A.guess(q0);
+    b <- A.guess(q0);
     return b;
   }
 }.
 
-(* TODO: ROM again *)
+clone ROM as MyROM with
+  type in_t <- Mblock,
+  type out_t <- C,
+  op dout <- fun (x:Mblock), CTS.dunifin
+proof *.
 
-clone ROM.Lazy as MyROM with
-  type from <- Mblock,
-  type to <- C,
-  op dsample <- fun (x:Mblock), unif<:C>.
-
-module RO = MyROM.RO.
+module RO = MyROM.Lazy.LRO.
 
 module PRFOracleRO:PRFOracleT = {
   var max_q:int
@@ -88,11 +99,11 @@ module PRFOracleRO:PRFOracleT = {
 
   proc queryPRF(m): C = {
     var r;
-    if (num_q >= max_q) {
-      r = witness;
+    if (max_q <= num_q) {
+      r <- witness;
     } else {
-      num_q = num_q + 1;
-      r = RO.o(m);
+      num_q <- num_q + 1;
+      r <- RO.o(m);
     }      
     return r;
   }
@@ -107,18 +118,17 @@ module PRF_Game2(A : AdvPRF) = {
   proc main(q0:int) : bool = {
     var b;
     RO.init();
-    PRFOracleRO.max_q = q0;
-    PRFOracleRO.num_q = 0;
+    PRFOracleRO.max_q <- q0;
+    PRFOracleRO.num_q <- 0;
     
-    b = A.guess(q0);
+    b <- A.guess(q0);
     return b;
   }
 }.
-
 (*
 axiom PRF (A<:AdvPRF{PRFOracle}) q &m:
   polytime A => poly q =>
-  | Pr[PRF_Game1(A).main(q) @ &m : res] - Pr[PRF_Game2(A).main(q) @ &m : res] | <= small.
+  | Pr[Game1(A).main(q) @ &m : res] - Pr[Game2(A).main(q) @ &m : res] | <= small.
 *)
 
 
@@ -134,7 +144,7 @@ module type AdvCR = {
 module CR(A:AdvCR) = {
   proc main(): bool= {
     var x,x':M;
-    (x,x') = A.adv();
+    (x,x') <- A.adv();
     return H x = H x' /\ x<>x';
   }
 }.
@@ -157,17 +167,17 @@ module type MacOracleT = {
 
 module MacOracle:MacOracleT = {
   var k:K
-  var max_q:int (* Max number of queries *)
+  var max_q:int  (* Max number of queries *)
   var msgLog: Mblock list
 
   proc query(m:Mblock) : C = {
       var r;
-      if (length msgLog >= max_q) {
-        r = witness;
+      if (max_q <= size msgLog) {
+        r <- witness;
       }
       else {
-        msgLog = m :: msgLog;
-        r = mac k m;
+        msgLog <- m :: msgLog;
+        r <- mac k m;
       }
       
       return r;
@@ -175,7 +185,7 @@ module MacOracle:MacOracleT = {
 }.
 
 module type AdvEFCMA (O:MacOracleT) = {
-  proc guess() : Mblock*C
+  proc guess () : Mblock*C
 }.
 
 module EF_CMA_Game (A : AdvEFCMA) = {
@@ -183,16 +193,18 @@ module EF_CMA_Game (A : AdvEFCMA) = {
   
   proc main (q0:int): bool = {
     var m', t';
-    MacOracle.k = $ unif;
-    MacOracle.max_q = q0;
-    MacOracle.msgLog = [];
+    MacOracle.k <$ KS.dunifin;
+    MacOracle.max_q <- q0;
+    MacOracle.msgLog <- [];
     
-    (m',t') = A.guess();
-    return (! mem m' MacOracle.msgLog) /\ (mac MacOracle.k m' = t');
+    (m',t') <- A.guess ();
+    return (! m' \in MacOracle.msgLog) /\ (mac MacOracle.k m' = t');
   }
 }.
 
 (*
+Comments from old lecture.
+
 (* Bad axiom: A may access the global variables of MacOracle!
    (In particular, access the key, or clear msgLog) *)
 axiom onetime_EFCMA (A<:AdvEFCMA) q &m:
@@ -223,14 +235,22 @@ axiom EFCMA (A<:AdvEFCMA{MacOracle}) q &m:
 *)
 
 
-
+(* ======================================================================= *)
 
 section. (* This keyword starts a section in which we can fix an
 adversary "once and for all", so that we do not need to quantify over
 it in each lemma *)
 
-declare module A : AdvEFCMA{MacOracle,PRFOracle,PRFOracleRO}. 
+declare module A <: AdvEFCMA{MacOracle,PRFOracle}. 
   (* Here we pick an adversary *)
+
+
+(* Problem 1: Define an adversary B such that the lemmas same_ora and
+step1 below are true. 
+
+(The source code of B must not contain the function "mac" directly,
+nor must it access any variables of O directly.) *)
+
 
 
 local module B(O:PRFOracleT) = {
@@ -240,12 +260,12 @@ local module B(O:PRFOracleT) = {
 
     proc query(m:Mblock) : C = {
     var r;
-    if (length msgLog >= max_q) {
-        r = witness;
+    if ( max_q <= size msgLog) {
+        r <- witness;
       }
       else {
-        msgLog = m :: msgLog;
-        r = O.queryPRF(m);
+        msgLog <- m :: msgLog;
+        r <- O.queryPRF(m);
       }
       
       return r;
@@ -265,38 +285,60 @@ local module B(O:PRFOracleT) = {
 
   proc guess(q:int): bool = { 
     var m', t', t'';
-    MacOra.msgLog = [];
-    MacOra.max_q = q-1;
-    (m',t') = A.guess();
+    MacOra.msgLog <- [];
+    MacOra.max_q <- q-1;
+    (m',t') <- A.guess();
 
-    t'' = O.queryPRF(m');
-    return (! mem m' MacOra.msgLog) /\ (t'' = t'); 
+    t'' <- O.queryPRF(m');
+    return (! m' \in MacOra.msgLog) /\ (t'' = t'); 
   }
 }.
-
+(* #POINTS 3 *)
 
 (* This lemma states that, give same input, the two Mac-oracles behave
 the same, and additionally they preserve a specific inveriant I *)
+
+(*  Problem 2: Prove this lemma.
+
+    Hint: You may find the tactic "if" useful, which makes a case
+    distinction over the condition of the first statement (assumed to
+    be an "if").
+
+    Hint: The lemma should be relatively simple to prove. If you need
+    fancy tools, probably your definitions above are incorrect.
+*)
 
 
 local lemma same_ora:
     equiv [ MacOracle.query ~ B(PRFOracle).MacOra.query : 
       ={m} /\
     (* Invariant I: *) (MacOracle.msgLog{1}=B.MacOra.msgLog{2} /\ MacOracle.max_q{1}=B.MacOra.max_q{2}
-               /\ (length B.MacOra.msgLog=PRFOracle.num_q /\ B.MacOra.max_q<PRFOracle.max_q){2}
-               /\ (PRFOracle.num_q < PRFOracle.max_q){2}
+               /\ (size B.MacOra.msgLog=PRFOracle.num_q /\ B.MacOra.max_q<PRFOracle.max_q){2}
+        /\ (PRFOracle.num_q < PRFOracle.max_q){2}
                /\ PRFOracle.f{2}=mac MacOracle.k{1})
       ==> ={res} /\ (MacOracle.msgLog{1}=B.MacOra.msgLog{2} /\ MacOracle.max_q{1}=B.MacOra.max_q{2}
-               /\ (length B.MacOra.msgLog=PRFOracle.num_q /\ B.MacOra.max_q<PRFOracle.max_q){2}
-               /\ (PRFOracle.num_q < PRFOracle.max_q){2}
+               /\ (size B.MacOra.msgLog=PRFOracle.num_q /\ B.MacOra.max_q<PRFOracle.max_q){2}
+        /\ (PRFOracle.num_q < PRFOracle.max_q){2}
                /\ PRFOracle.f{2}=mac MacOracle.k{1}) ].
 proc.
 if => //.
 by auto.
 inline *.
 auto.
-timeout 9. smt.
+smt.
 qed.
+
+(* #POINTS 3 *)
+
+
+(*  Problem 3: Prove this lemma.
+
+    This one is tricky. If you get stuck on an smt-goal, try
+    progress. progress splits your goal into lots of small goals.  Try
+    solving each with smt. If one of them is not solvable, that
+    probably indicates where the problem lies.
+
+*)
 
 
 (* This lemma states that the two games behave the same. Note that we
@@ -304,56 +346,62 @@ run the second game with one more query. This is because the adversary
 B needs to make one extra call to the PRF to check the tag t *)
 
 local lemma step1 &m q:
-    q >= 0 =>
+    0 <= q =>
     Pr[ EF_CMA_Game(A).main(q) @ &m : res ] = Pr [ PRF_Game1(B).main(q+1) @ &m : res].
 proof.
-intros q_nat.
+move => q_nat.
 byequiv => //.
 proc.
+inline PRF_Game1(B).A.guess.
 inline *.
 wp.
-conseq (_: ={glob A} /\ q0{1}+1=q0{2} /\ q0{1} >= 0
+conseq (_: ={glob A} /\ q0{1}+1=q0{2} /\ 0 <= q0{1}
   ==> ={m',t'} /\ MacOracle.msgLog{1}=B.MacOra.msgLog{2}
       /\ mac MacOracle.k{1}=PRFOracle.f{2}
-      /\ PRFOracle.num_q{2} < PRFOracle.max_q{2}). smt.  progress; smt.
+      /\ PRFOracle.num_q{2} < PRFOracle.max_q{2}). smt.  smt.
 call (_: MacOracle.msgLog{1}=B.MacOra.msgLog{2} /\ MacOracle.max_q{1}=B.MacOra.max_q{2}
-               /\ (length B.MacOra.msgLog=PRFOracle.num_q /\ B.MacOra.max_q<PRFOracle.max_q){2}
+               /\ (size B.MacOra.msgLog=PRFOracle.num_q /\ B.MacOra.max_q<PRFOracle.max_q){2}
                /\ (PRFOracle.num_q < PRFOracle.max_q){2}
                /\ PRFOracle.f{2}=mac MacOracle.k{1}).
 by apply same_ora.
 conseq (_: _ ==>
      ={glob A} /\ MacOracle.msgLog{1}=B.MacOra.msgLog{2} /\ MacOracle.max_q{1}=B.MacOra.max_q{2}
-               /\ (length B.MacOra.msgLog=PRFOracle.num_q /\ B.MacOra.max_q<PRFOracle.max_q){2}
+               /\ (size B.MacOra.msgLog=PRFOracle.num_q /\ B.MacOra.max_q<PRFOracle.max_q){2}
                /\ (PRFOracle.num_q < PRFOracle.max_q){2}
                /\ PRFOracle.f{2}=mac MacOracle.k{1}).
 smt.
 wp.
-conseq (_: _ ==> ={glob A} /\ MacOracle.k{1} = k{2} /\ q0{1} >= 0 /\ q0{1}+1 = q0{2}).
-progress; smt.
+conseq (_: _ ==> ={glob A} /\ MacOracle.k{1} = k{2} /\0 <=  q0{1} /\ q0{1}+1 = q0{2}).
+smt.
 rnd.
 auto.
 qed.
 
-
 (* ================= START ================= *)
 
-op cardC = FSet.card (ISet.Finite.toFSet univ<:C>).
+op cardC = CTS.Support.card.
 
 (* Some useful lemma *)
 lemma cardC_pos: 1%r/cardC%r >= 0%r.
     admit.
 qed.
 
+print CTS.dunifin1E.
+
 (* Some useful lemma *)
-lemma card_pr t': mu unif (fun (y : C) => y = t') = 1%r / cardC%r.
-proof.
-  rewrite (_: (fun (y : C) => y = t') = (=) t').
-    admit. (* apply fun_ext; smt. *)
-  rewrite -/mu_x.
-  cut H1: mu_x unif t' = 1%r / cardC%r.
-    smt.
-  smt.
-qed.
+(*
+TODO: Since we clone finite, we already get this lemma for "free"
+We can do away with this lemma.
+*)
+
+(* lemma card_pr t': mu CTS.dunifin (fun (y : C) => y = t') = 1%r / cardC%r. *)
+(* proof. *)
+(*   rewrite (_: (fun (y : C) => y = t') = (=) t'). *)
+(*   apply fun_ext; smt. *)
+(*   have H1: mu_x CTS.dunifin t' = 1%r / cardC%r. *)
+(*     smt. *)
+(*   smt. *)
+(* qed. *)
 
 
 
@@ -383,15 +431,17 @@ qed.
 
 *)
 
+(* TODO: FMap.Dom, and RO.m  *)
+
 local lemma query_inv:
   hoare [ B(PRFOracleRO).MacOra.query : 
             B.MacOra.max_q < PRFOracleRO.max_q
-            /\ FMap.dom RO.m = FSet.of_list B.MacOra.msgLog
+            /\ FMap.dom RO.m = FSet.oflist B.MacOra.msgLog
             /\ length B.MacOra.msgLog <= B.MacOra.max_q         
             /\ PRFOracleRO.num_q = length B.MacOra.msgLog
         ==>
             B.MacOra.max_q < PRFOracleRO.max_q
-            /\ FMap.dom RO.m = FSet.of_list B.MacOra.msgLog
+            /\ FMap.dom RO.m = FSet.oflist B.MacOra.msgLog
             /\ length B.MacOra.msgLog <= B.MacOra.max_q         
             /\ PRFOracleRO.num_q = length B.MacOra.msgLog ].
 proof.
@@ -436,13 +486,13 @@ proof.
   inline PRF_Game2(B).A.guess.
   seq 7: (true) 1%r (1%r/cardC%r) 0%r _
          (PRFOracleRO.num_q < PRFOracleRO.max_q
-            /\ FMap.dom RO.m = FSet.of_list B.MacOra.msgLog) => //.
+            /\ FMap.dom RO.m = FSet.oflist B.MacOra.msgLog) => //.
   
   (* Two subgoals left at this point *)
 
   (* Invariant is satisfied after first half of game *)
   call (_: B.MacOra.max_q < PRFOracleRO.max_q
-            /\ FMap.dom RO.m = FSet.of_list B.MacOra.msgLog
+            /\ FMap.dom RO.m = FSet.oflist B.MacOra.msgLog
             /\ length B.MacOra.msgLog <= B.MacOra.max_q         
             /\ PRFOracleRO.num_q = length B.MacOra.msgLog).
     by apply query_inv.
